auto_generated/coq/abis.v
@@ -179,7 +179,7 @@ Definition anyAbiFeatureTagEquiv  (f1 : any_abi_feature ) (f2 : any_abi_feature 
        |(Aarch64LeAbiFeature(af1),  Aarch64LeAbiFeature(af2)) => abiFeatureTagEq af1 af2
     end.
 
-Instance x116_Ord : Ord any_abi_feature := {
+Instance x117_Ord : Ord any_abi_feature := {
      compare  :=  anyAbiFeatureCompare;
      isLess  :=  fun  f1 => (fun  f2 => ( (ordering_equal (anyAbiFeatureCompare f1 f2) LT)));
      isLessEqual  :=  fun  f1 => (fun  f2 => (set_member_by (fun  x  y=>EQ) (anyAbiFeatureCompare f1 f2) [LT;  EQ]));
@@ -188,7 +188,7 @@ Instance x116_Ord : Ord any_abi_feature := {
 }.
 
 
-Instance x115_AbiFeatureTagEquiv : AbiFeatureTagEquiv any_abi_feature := {
+Instance x116_AbiFeatureTagEquiv : AbiFeatureTagEquiv any_abi_feature := {
      abiFeatureTagEquiv  :=  anyAbiFeatureTagEquiv
 }.
 
@@ -223,95 +223,104 @@ Definition make_elf64_header  (data : nat ) (osabi : nat ) (abiv : nat ) (ma : n
        |}.
 (* [?]: removed value specification. *)
 
-Definition make_load_phdrs {abifeature : Type}  (max_page_sz : nat ) (common_page_sz : nat ) (img3 : annotated_memory_image abifeature) (section_pairs_bare_sorted_by_address : list (elf64_interpreted_section ))  : list (elf64_program_header_table_entry ):=  
-    let phdr_flags_from_section_flags := fun (section_flags : nat ) => fun (sec_name : string ) =>
-        let flags := nat_lor elf_pf_r (nat_lor 
-            (if flag_is_set shf_write section_flags then elf_pf_w else 0)
-            (if flag_is_set shf_execinstr section_flags then elf_pf_x else 0))
-        in
-        (*let _ = errln ("Phdr flags of section " ^ sec_name ^ "(ELF section flags 0x " ^ 
-            (hex_string_of_natural section_flags) ^ ") are 0x" ^ (hex_string_of_natural flags))
-        in*)
-        flags
+Definition phdr_flags_from_section_flags  (section_flags : nat ) (sec_name : string )  : nat := 
+    let flags := nat_lor elf_pf_r (nat_lor 
+        (if flag_is_set shf_write section_flags then elf_pf_w else 0)
+        (if flag_is_set shf_execinstr section_flags then elf_pf_x else 0))
     in
-    let maybe_extend_phdr := fun (phdr : elf64_program_header_table_entry ) => fun (isec1 : elf64_interpreted_section ) => ( 
-        let new_p_type := nat_of_elf64_word(elf64_p_type phdr)
-        in
-        let this_section_phdr_flags := phdr_flags_from_section_flags(elf64_section_flags isec1)(elf64_section_name_as_string isec1)
-        in
-        let can_combine_flags := fun (flagsets : set (nat )) => 
-            (* The GNU linker happily adds a .rodata section to a RX segment,
-             * but not to a RW segment. So the only clear rule is: if any is writable,
-             * all must be writable. *)
-            let is_writable := fun (flags : nat ) => beq_nat (nat_land flags elf_pf_w) elf_pf_w
-            in
-            let flagslist := set_to_list flagsets
-            in
-            let union_flags := List.fold_left nat_lor flagslist ( 0)
-            in
-            if List.existsb is_writable flagslist
-            then
-                if List.forallb is_writable flagslist then Some union_flags
-                else None
-            else
-                Some union_flags
-        in
-        let maybe_extended_flags := can_combine_flags [ this_section_phdr_flags;  nat_of_elf64_word(elf64_p_flags phdr) ]
-        in
-        if (maybeEqualBy beq_nat maybe_extended_flags None) then (*let _ = errln "flag mismatch" in*) None
-        else let new_p_flags := match ( maybe_extended_flags) with  Some flags => flags | _ => DAEMON end
-        in
-        (* The new filesz is the file end offset of this section,
-         * minus the existing file start offset of the phdr. 
-         * Check that the new section begins after the old offset+filesz. *)
-        if nat_ltb(elf64_section_offset isec1) (Coq.Init.Peano.plus (nat_of_elf64_off(elf64_p_offset phdr)) (nat_of_elf64_xword(elf64_p_filesz phdr)))
-        then (*let _ = errln "offset went backwards" in*) None
-        else 
-        let new_p_filesz := Coq.Init.Peano.plus (nat_of_elf64_xword(elf64_p_filesz phdr)) (if beq_nat(elf64_section_type isec1) sht_progbits then(elf64_section_size isec1) else 0)
-        in 
-        (* The new memsz is the virtual address end address of this section,
-         * minus the existing start vaddr of the phdr. 
-         * Check that the new section begins after the old vaddr+memsz. *)
-        if nat_ltb(elf64_section_addr isec1) (Coq.Init.Peano.plus (nat_of_elf64_addr(elf64_p_vaddr phdr)) (nat_of_elf64_xword(elf64_p_memsz phdr)))
-        then (*let _ = errln "vaddr went backwards" in*) None
-        else 
-        let new_p_memsz := Coq.Init.Peano.plus (nat_of_elf64_xword(elf64_p_memsz phdr))(elf64_section_size isec1)
-        in
-        let one_if_zero := fun (n : nat ) => if beq_nat n( 0) then 1 else n
-        in
-        let new_p_align :=  lcm (one_if_zero (nat_of_elf64_xword(elf64_p_align phdr))) (one_if_zero(elf64_section_align isec1))
-        in
-        Some
-          {|elf64_p_type   := (elf64_word_of_nat new_p_type)
-           ;elf64_p_flags  := (elf64_word_of_nat new_p_flags)
-           ;elf64_p_offset :=(elf64_p_offset phdr)
-           ;elf64_p_vaddr  :=(elf64_p_vaddr phdr)
-           ;elf64_p_paddr  :=(elf64_p_paddr phdr)
-           ;elf64_p_filesz := (elf64_xword_of_nat new_p_filesz)
-           ;elf64_p_memsz  := (elf64_xword_of_nat new_p_memsz)
-           ;elf64_p_align  := (elf64_xword_of_nat new_p_align)
-           |}
-    )
+    (*let _ = errln ("Phdr flags of section " ^ sec_name ^ "(ELF section flags 0x " ^ 
+        (hex_string_of_natural section_flags) ^ ") are 0x" ^ (hex_string_of_natural flags))
+    in*)
+    flags.
+(* [?]: removed value specification. *)
+
+Definition phdr_is_writable  (flags : nat )  : bool :=  beq_nat
+    (nat_land flags elf_pf_w) elf_pf_w.
+
+Definition can_combine_flags_fn : Type :=  set  nat  ->  option  nat  .
+Definition can_combine_flags_fn_default: can_combine_flags_fn  := (fun (x115 :  set  nat ) => DAEMON).
+(* [?]: removed value specification. *)
+
+Definition load_can_combine_flags  (flagsets : set (nat ))  : option (nat ) :=  
+    (* The GNU linker happily adds a .rodata section to a RX segment,
+     * but not to a RW segment. So the only clear rule is: if any is writable,
+     * all must be writable. *)
+    let flagslist := set_to_list flagsets
     in
-    let rounded_down_offset := fun (isec1 : elf64_interpreted_section ) => round_down_to common_page_sz(elf64_section_offset isec1)
+    let union_flags := List.fold_left nat_lor flagslist ( 0)
+    in
+    if List.existsb phdr_is_writable flagslist
+    then
+        if List.forallb phdr_is_writable flagslist then Some union_flags
+        else None
+    else
+        Some union_flags.
+(* [?]: removed value specification. *)
+
+Definition tls_can_combine_flags  (flagsets : set (nat ))  : option (nat ) :=  Some (List.fold_left nat_lor (set_to_list flagsets) ( 0)).
+
+Definition maybe_extend_phdr  (phdr : elf64_program_header_table_entry ) (isec1 : elf64_interpreted_section ) (can_combine_flags : set (nat ) -> option (nat ) )  : option (elf64_program_header_table_entry ) := 
+    let new_p_type := nat_of_elf64_word(elf64_p_type phdr)
+    in
+    let this_section_phdr_flags := phdr_flags_from_section_flags(elf64_section_flags isec1)(elf64_section_name_as_string isec1)
+    in
+    let maybe_extended_flags := can_combine_flags [ this_section_phdr_flags;  nat_of_elf64_word(elf64_p_flags phdr) ]
+    in
+    if (maybeEqualBy beq_nat maybe_extended_flags None) then (*let _ = errln "flag mismatch" in*) None
+    else let new_p_flags := match ( maybe_extended_flags) with  Some flags => flags | _ => DAEMON end
+    in
+    (* The new filesz is the file end offset of this section,
+     * minus the existing file start offset of the phdr. 
+     * Check that the new section begins after the old offset+filesz. *)
+    if nat_ltb(elf64_section_offset isec1) (Coq.Init.Peano.plus (nat_of_elf64_off(elf64_p_offset phdr)) (nat_of_elf64_xword(elf64_p_filesz phdr)))
+    then (*let _ = errln "offset went backwards" in*) None
+    else 
+    let new_p_filesz := Coq.Init.Peano.plus (nat_of_elf64_xword(elf64_p_filesz phdr)) (if beq_nat(elf64_section_type isec1) sht_progbits then(elf64_section_size isec1) else 0)
+    in 
+    (* The new memsz is the virtual address end address of this section,
+     * minus the existing start vaddr of the phdr. 
+     * Check that the new section begins after the old vaddr+memsz. *)
+    if nat_ltb(elf64_section_addr isec1) (Coq.Init.Peano.plus (nat_of_elf64_addr(elf64_p_vaddr phdr)) (nat_of_elf64_xword(elf64_p_memsz phdr)))
+    then (*let _ = errln "vaddr went backwards" in*) None
+    else 
+    let new_p_memsz := Coq.Init.Peano.plus (nat_of_elf64_xword(elf64_p_memsz phdr))(elf64_section_size isec1)
+    in
+    let one_if_zero := fun (n : nat ) => if beq_nat n( 0) then 1 else n
+    in
+    let new_p_align :=  lcm (one_if_zero (nat_of_elf64_xword(elf64_p_align phdr))) (one_if_zero(elf64_section_align isec1))
+    in
+    Some
+      {|elf64_p_type   := (elf64_word_of_nat new_p_type)
+       ;elf64_p_flags  := (elf64_word_of_nat new_p_flags)
+       ;elf64_p_offset :=(elf64_p_offset phdr)
+       ;elf64_p_vaddr  :=(elf64_p_vaddr phdr)
+       ;elf64_p_paddr  :=(elf64_p_paddr phdr)
+       ;elf64_p_filesz := (elf64_xword_of_nat new_p_filesz)
+       ;elf64_p_memsz  := (elf64_xword_of_nat new_p_memsz)
+       ;elf64_p_align  := (elf64_xword_of_nat new_p_align)
+       |}.
+
+Definition make_new_phdr  (isec1 : elf64_interpreted_section ) (t : nat ) (maxpagesize1 : nat ) (commonpagesize1 : nat )  : elf64_program_header_table_entry := 
+    let rounded_down_offset := fun (isec1 : elf64_interpreted_section ) => round_down_to commonpagesize1(elf64_section_offset isec1)
     in
     let offset_round_down_amount := fun (isec1 : elf64_interpreted_section ) => Coq.Init.Peano.minus(elf64_section_offset isec1) (rounded_down_offset isec1)
     in
-    let rounded_down_vaddr := fun (isec1 : elf64_interpreted_section ) => round_down_to common_page_sz(elf64_section_addr isec1)
+    let rounded_down_vaddr := fun (isec1 : elf64_interpreted_section ) => round_down_to commonpagesize1(elf64_section_addr isec1)
     in
     let vaddr_round_down_amount := fun (isec1 : elf64_interpreted_section ) => Coq.Init.Peano.minus(elf64_section_addr isec1) (rounded_down_vaddr isec1)
     in
-    let new_phdr := fun (isec1 : elf64_interpreted_section ) => 
-      {|elf64_p_type   := (elf64_word_of_nat elf_pt_load) (** Type of the segment *)
-       ;elf64_p_flags  := (elf64_word_of_nat (phdr_flags_from_section_flags(elf64_section_flags isec1)(elf64_section_name_as_string isec1))) (** Segment flags *)
-       ;elf64_p_offset := (elf64_off_of_nat (rounded_down_offset isec1)) (** Offset from beginning of file for segment *)
-       ;elf64_p_vaddr  := (elf64_addr_of_nat (rounded_down_vaddr isec1)) (** Virtual address for segment in memory *)
-       ;elf64_p_paddr  := (elf64_addr_of_nat( 0)) (** Physical address for segment *)
-       ;elf64_p_filesz := (elf64_xword_of_nat (if beq_nat(elf64_section_type isec1) sht_nobits then 0 else Coq.Init.Peano.plus(elf64_section_size isec1) (offset_round_down_amount isec1))) (** Size of segment in file, in bytes *)
-       ;elf64_p_memsz  := (elf64_xword_of_nat ( Coq.Init.Peano.plus(elf64_section_sizeisec1) (vaddr_round_down_amount isec1))) (** Size of segment in memory image, in bytes *)
-       ;elf64_p_align  := (elf64_xword_of_nat (* isec.elf64_section_align *) max_page_sz) (** Segment alignment memory for memory and file *)
-       |}
-    in
+  {|elf64_p_type   := (elf64_word_of_nat t) (** Type of the segment *)
+   ;elf64_p_flags  := (elf64_word_of_nat (phdr_flags_from_section_flags(elf64_section_flags isec1)(elf64_section_name_as_string isec1))) (** Segment flags *)
+   ;elf64_p_offset := (elf64_off_of_nat (rounded_down_offset isec1)) (** Offset from beginning of file for segment *)
+   ;elf64_p_vaddr  := (elf64_addr_of_nat (rounded_down_vaddr isec1)) (** Virtual address for segment in memory *)
+   ;elf64_p_paddr  := (elf64_addr_of_nat( 0)) (** Physical address for segment *)
+   ;elf64_p_filesz := (elf64_xword_of_nat (if beq_nat(elf64_section_type isec1) sht_nobits then 0 else Coq.Init.Peano.plus(elf64_section_size isec1) (offset_round_down_amount isec1))) (** Size of segment in file, in bytes *)
+   ;elf64_p_memsz  := (elf64_xword_of_nat ( Coq.Init.Peano.plus(elf64_section_sizeisec1) (vaddr_round_down_amount isec1))) (** Size of segment in memory image, in bytes *)
+   ;elf64_p_align  := (elf64_xword_of_nat (* isec.elf64_section_align *) maxpagesize1) (** Segment alignment memory for memory and file *)
+   |}.
+(* [?]: removed value specification. *)
+
+Definition make_load_phdrs {abifeature : Type}  (maxpagesize1 : nat ) (commonpagesize1 : nat ) (img3 : annotated_memory_image abifeature) (section_pairs_bare_sorted_by_address : list (elf64_interpreted_section ))  : list (elf64_program_header_table_entry ):=  
     (* accumulate sections into the phdr *)
     let rev_list := List.fold_left (fun (accum_phdr_list : list (elf64_program_header_table_entry )) => (fun (isec1 : elf64_interpreted_section ) => (
         (* Do we have a current phdr? *)
@@ -319,14 +328,14 @@ Definition make_load_phdrs {abifeature : Type}  (max_page_sz : nat ) (common_pag
             [] => (* no, so make one *)
                 (*let _ = errln ("Starting the first LOAD phdr for section " ^ isec.elf64_section_name_as_string)
                 in*)
-                [new_phdr isec1]
+                [make_new_phdr isec1 elf_pt_load maxpagesize1 commonpagesize1]
             | current_phdr :: more => 
                 (* can we extend it with the current section? *)
-                match ( maybe_extend_phdr current_phdr isec1) with 
+                match ( maybe_extend_phdr current_phdr isec1 load_can_combine_flags) with 
                     None => 
                         (*let _ = errln ("Starting new LOAD phdr for section " ^ isec.elf64_section_name_as_string)
                         in*)
-                        (new_phdr isec1) :: (current_phdr :: more)
+                        (make_new_phdr isec1 elf_pt_load maxpagesize1 commonpagesize1) :: (current_phdr :: more)
                     | Some phdr => phdr :: more
                 end
         end
@@ -336,6 +345,43 @@ Definition make_load_phdrs {abifeature : Type}  (max_page_sz : nat ) (common_pag
     (*let _ = errln "Successfully made phdrs"
     in*)
     List.rev rev_list.
+(* [?]: removed value specification. *)
+
+Definition tls_extend {abifeature : Type}  (a : abi abifeature)  : abi abifeature:=  
+   {|is_valid_elf_header :=(is_valid_elf_header a)
+    ;make_elf_header     :=(make_elf_header a)
+    ;reloc               :=(reloc a)
+    ;section_is_special  :=(section_is_special a)
+    ;section_is_large    :=(section_is_large a)
+    ;maxpagesize         :=(maxpagesize a)
+    ;minpagesize         :=(minpagesize a)
+    ;commonpagesize      :=(commonpagesize a)
+    ;symbol_is_generated_by_linker :=(symbol_is_generated_by_linker a)
+    ;make_phdrs          := (fun (maxpagesize1 : nat ) => fun (commonpagesize1 : nat ) => fun (file_type : nat ) => fun (img3 : annotated_memory_image abifeature) => fun (section_pairs_bare_sorted_by_address : list (elf64_interpreted_section )) => (
+        let rev_list := List.fold_left (fun (accum_phdr_list : list (elf64_program_header_table_entry )) => (fun (isec1 : elf64_interpreted_section ) => (
+        match ( accum_phdr_list) with 
+            [] =>
+                (*let _ = errln "Making a new TLS program header" in *)
+                [make_new_phdr isec1 elf_pt_tls maxpagesize1 commonpagesize1]
+            | current_phdr :: more => 
+                match ( maybe_extend_phdr current_phdr isec1 tls_can_combine_flags) with 
+                    None => 
+                        (make_new_phdr isec1 elf_pt_tls maxpagesize1 commonpagesize1) :: (current_phdr :: more)
+                    | Some phdr => phdr :: more
+                end
+        end
+        ))) (List.filter (fun (isec1 : elf64_interpreted_section ) => flag_is_set shf_alloc(elf64_section_flags isec1)
+            && flag_is_set shf_tls(elf64_section_flags isec1)) section_pairs_bare_sorted_by_address) []
+        in
+         (@ List.app _)((make_phdrsa) maxpagesize1 commonpagesize1 file_type img3 section_pairs_bare_sorted_by_address) (List.rev rev_list)
+    ))
+    ;max_phnum           := (Coq.Init.Peano.plus( 1)(max_phnum a))
+    ;guess_entry_point   :=(guess_entry_point a)
+    ;pad_data            :=(pad_data a)
+    ;pad_code            :=(pad_code a)
+    ;generate_support    :=(generate_support a)
+    ;concretise_support  :=(concretise_support a)
+    |}.
 (* [?]: removed value specification. *)
 
 Definition make_default_phdrs {abifeature : Type}  (maxpagesize1 : nat ) (commonpagesize1 : nat ) (t : nat ) (img3 : annotated_memory_image abifeature) (section_pairs_bare_sorted_by_address : list (elf64_interpreted_section ))  : list (elf64_program_header_table_entry ):=  
@@ -376,10 +422,10 @@ Definition find_start_symbol_address {abifeature : Type} `{Ord abifeature} `{Abi
     end.
 (* [?]: removed value specification. *)
 
-Definition pad_zeroes  (n : nat )  : list (byte ):=  replicate0 n (byte_of_nat( 0)).
+Definition pad_zeroes  (n : nat )  : list (elf_types_local.byte ):=  replicate0 n (byte_of_nat( 0)).
 (* [?]: removed value specification. *)
 
-Definition pad_0x90  (n : nat )  : list (byte ):=  replicate0 n (byte_of_nat ( Coq.Init.Peano.mult( 9)( 16))).
+Definition pad_0x90  (n : nat )  : list (elf_types_local.byte ):=  replicate0 n (byte_of_nat ( Coq.Init.Peano.mult( 9)( 16))).
 (* [?]: removed value specification. *)
  
 Definitionnull_abi   : abi (any_abi_feature ):=  {|is_valid_elf_header := is_valid_elf64_header
@@ -438,7 +484,7 @@ Definition amd64_generate_support  (input_fnames_and_imgs : list ((string *annot
                                       (* Is this ref a relocation we're going to apply, and does it reference the GOT? *)
                                       match ( ((maybe_relocrr),(maybe_def_bound_to rr))) with
                                           (None,  _) => None
-                                        | (Some r,  Some(ApplyReloc,  maybe_def)) =>
+                                        | (Some r,  Some(ApplyReloc(_),  maybe_def)) =>
                                         if ( (set_member_by
                                                 (genericCompare nat_ltb
                                                    beq_nat)
@@ -454,9 +500,7 @@ Definition amd64_generate_support  (input_fnames_and_imgs : list ((string *annot
                                         else None
                                         | (Some r,  Some(MakePIC,  maybe_def)) =>
                                         DAEMON | (Some _, None) =>
-                                        DAEMON (* Incomplete Pattern at File \"abis/abis.lem\", line 356, character 13 to line 366, character 15 *)
-                                        | (Some _, Some(LeaveReloc,  _)) =>
-                                        DAEMON (* Incomplete Pattern at File \"abis/abis.lem\", line 356, character 13 to line 366, character 15 *)
+                                        DAEMON (* Incomplete Pattern at File \"abis/abis.lem\", line 403, character 13 to line 413, character 15 *)
                                       end | _ => DAEMON end end)
                                tags_and_ranges end) tags_and_ranges_by_image
   in
@@ -495,7 +539,15 @@ Definition amd64_generate_support  (input_fnames_and_imgs : list ((string *annot
                       (Some
                          (".got", ( 0, Coq.Init.Peano.mult nentries entrysize)), 
                       AbiFeature
-                        (Amd64AbiFeature (abi_amd64.GOT0 (refs_via_got))))
+                        (Amd64AbiFeature
+                           (abi_amd64.GOT0
+                              (set_to_list
+                                 ((set_from_list_by
+                                     (pairCompare
+                                        (fun (x : string ) (y : string )=> EQ)
+                                        (maybeCompare
+                                           (fun (x : symbol_definition ) (y : symbol_definition )=>
+                                              EQ))) refs_via_got))))))
                       ;  (Some
                             (".got", ( 0, Coq.Init.Peano.mult nentries
                                             entrysize)), FileFeature
@@ -577,14 +629,15 @@ Definition amd64_concretise_support  (img3 : annotated_memory_image (any_abi_fea
                       | [((def_el_name,  (def_start,  def_len)),  d)] =>
                       match ( element_and_offset_to_address
                                 (def_el_name, def_start) img3) with None =>
-                        DAEMON | Some addr =>
+                        DAEMON | Some x =>
                         (*let _ = errln ("GOT slot for symbol `" ^ symname ^ 
-                                                "' created pointing to address 0x" ^ (hex_string_of_natural addr) ^ 
+                                                "' created pointing to address 0x" ^ (hex_string_of_natural x) ^ 
                                                 " (offset 0x" ^ (hex_string_of_natural def_start) ^ " in element " ^ def_el_name ^ ")")
                                             in*)
-                      addr end | _ => DAEMON end end in
+                      x end | _ => DAEMON end end in
     let addr_bytes := natural_to_le_byte_list addr in
-    (@ List.app _) (List.map (fun (b : byte ) => Some b) addr_bytes)
+    (@ List.app _)
+      (List.map (fun (b : elf_types_local.byte ) => Some b) addr_bytes)
       (replicate0 ( Coq.Init.Peano.minus ( 8) (length addr_bytes))
          (Some (byte_of_nat ( 0)))) end
                     ) l
@@ -611,6 +664,115 @@ Definition amd64_concretise_support  (img3 : annotated_memory_image (any_abi_fea
                 | _ => DAEMON
             end
     end.
+(* [?]: removed value specification. *)
+
+Definition amd64_got_slot_idx  (img3 : annotated_memory_image (any_abi_feature )) (rr : symbol_reference_and_reloc_site )  : nat :=  
+    (*let _ = errln ("Looking up GOT slot for symbol " ^ rr.ref.ref_symname) in*)
+    match ( (fmap_lookup_by (fun (x : string ) (y : string )=>EQ) ".got"(elements img3))) with 
+        None => (* got no GOT? okay... *) DAEMON
+        | Some got_el => 
+            (* Find the GOT tag. *)
+            let tags_and_ranges := multimap.lookupBy0 memory_image_orderings.tagEquiv (AbiFeature(Amd64AbiFeature(abi_amd64.GOT0([]))))(by_tag img3)
+            in
+            match ( tags_and_ranges) with 
+                [] => DAEMON
+                | [(AbiFeature(Amd64AbiFeature(abi_amd64.GOT0(l))),  Some(got_el_name,  (got_start_off,  got_len)))] => 
+                    (* Find the slot corresponding to rr, if we have one. *)
+                    let got_addr := match ((startpos got_el)) with  Some addr => addr | None => DAEMON end
+                    in
+                    match ((maybe_def_bound_to rr)) with 
+                        Some (_,  Some(d)) => 
+                            match ( lem_list.findIndex (
+  fun (p : (string *option (symbol_definition ) ) % type) =>
+    match ( (p) ) with ( (symname,  maybe_def)) =>
+      (maybeEqualBy classical_boolean_equivalence (Some (d)) maybe_def) end) l) with 
+                                Some idx1 =>  idx1
+                             |  None => DAEMON
+                            end
+                        | Some(_,  None) => (* HACK: look for the weak symname. Really want more (ref-based) labelling. *)
+                            match ( lem_list.findIndex (
+  fun (p : (string *option (symbol_definition ) ) % type) =>
+    match ( (p) ) with ( (symname,  _)) =>
+      (string_equal symname (ref_symname(ref rr))) end) l) with 
+                                Some idx1 =>  idx1
+                             |  None => DAEMON
+                            end
+                        | _ => DAEMON
+                    end
+                | _ => DAEMON
+            end
+    end.
+(* [?]: removed value specification. *)
+
+Definition amd64_got_slot_addr  (img3 : annotated_memory_image (any_abi_feature )) (rr : symbol_reference_and_reloc_site )  : nat :=  
+    match ( (fmap_lookup_by (fun (x : string ) (y : string )=>EQ) ".got"(elements img3))) with 
+        None => (* got no GOT? okay... *) DAEMON
+        | Some got_el => 
+            (* Find the GOT tag. *)
+            let tags_and_ranges := multimap.lookupBy0 memory_image_orderings.tagEquiv (AbiFeature(Amd64AbiFeature(abi_amd64.GOT0([]))))(by_tag img3)
+            in
+            match ( tags_and_ranges) with 
+                [] => DAEMON
+                | [(AbiFeature(Amd64AbiFeature(abi_amd64.GOT0(l))),  Some(got_el_name,  (got_start_off,  got_len)))] => 
+                    (* Find the slot corresponding to rr, if we have one. *)
+                    let got_addr := match ((startpos got_el)) with  Some addr => addr | None => DAEMON end
+                    in Coq.Init.Peano.plus (Coq.Init.Peano.mult( 8) (amd64_got_slot_idx img3 rr)) got_addr
+                | _ => DAEMON
+            end
+    end.
+(* [?]: removed value specification. *)
+
+Definition amd64_reloc  (r : nat )  : (bool *(annotated_memory_image (any_abi_feature ) -> nat  -> symbol_reference_and_reloc_site  -> (nat *(nat  -> Z  -> nat  -> nat )) % type)) % type:=  
+    let n2i := (fun (n : nat )=>(Zpred (Zpos (P_of_succ_nat n)))) in 
+    let i2n := Zabs_nat in 
+    let i2n_signed := fun (width : nat ) => fun (i : Z ) => (
+        if int_gteb i((Zpred (Zpos (P_of_succ_nat 0)))) then 
+            if int_gteb i (Coq.ZArith.Zpower.Zpower_nat((Zpred (Zpos (P_of_succ_nat 2)))) (Coq.Init.Peano.minus width( 1))) then DAEMON
+            else Zabs_nat i
+        else 
+            (* We manually encode the 2's complement of the negated value *)
+            let negated := Zabs_nat ( Coq.ZArith.BinInt.Zminus((Zpred (Zpos (P_of_succ_nat 0)))) i) in 
+            let xormask := ( Coq.Init.Peano.minus (nat_power( 2) width)( 1)) in
+            let compl := Coq.Init.Peano.plus( 1) (nat_lxor negated xormask)
+            in compl
+    )
+    in
+    match ( (string_of_amd64_relocation_type r)) with 
+    | "R_X86_64_NONE" =>            (false, (fun (img3 : annotated_memory_image (any_abi_feature )) => (fun (site_addr : nat ) => (fun (rr : symbol_reference_and_reloc_site ) => ( 0, (fun (s : nat ) => fun (a : Z ) => fun (e : nat ) => e))))))
+    | "R_X86_64_64" =>              (true,  (fun (img3 : annotated_memory_image (any_abi_feature )) => (fun (site_addr : nat ) => (fun (rr : symbol_reference_and_reloc_site ) => ( 8, (fun (s : nat ) => fun (a : Z ) => fun (e : nat ) => i2n ( Coq.ZArith.BinInt.Zplus(n2i s) a)))))))
+    | "R_X86_64_PC32" =>            (false, (fun (img3 : annotated_memory_image (any_abi_feature )) => (fun (site_addr : nat ) => (fun (rr : symbol_reference_and_reloc_site ) => ( 4, (fun (s : nat ) => fun (a : Z ) => fun (e : nat ) => Coq.Init.Peano.minus (i2n ( Coq.ZArith.BinInt.Zplus(n2i s) a)) site_addr))))))
+    | "R_X86_64_GOT32" =>           (false, (fun (img3 : annotated_memory_image (any_abi_feature )) => (fun (site_addr : nat ) => (fun (rr : symbol_reference_and_reloc_site ) => ( 4, (fun (s : nat ) => fun (a : Z ) => fun (e : nat ) => i2n_signed( 32) ( Coq.ZArith.BinInt.Zplus(n2i (amd64_got_slot_idx img3 rr)) a)))))))
+    | "R_X86_64_PLT32" =>           (false, (fun (img3 : annotated_memory_image (any_abi_feature )) => (fun (site_addr : nat ) => (fun (rr : symbol_reference_and_reloc_site ) => ( 4, (fun (s : nat ) => fun (a : Z ) => fun (e : nat ) => e)) (* FIXME *)))))
+    | "R_X86_64_COPY" =>            (false, (fun (img3 : annotated_memory_image (any_abi_feature )) => (fun (site_addr : nat ) => (fun (rr : symbol_reference_and_reloc_site ) => (size_of_copy_reloc img3 rr, (fun (s : nat ) => fun (a : Z ) => fun (e : nat ) => e)) (* FIXME *)))))
+    | "R_X86_64_GLOB_DAT" =>        (false, (fun (img3 : annotated_memory_image (any_abi_feature )) => (fun (site_addr : nat ) => (fun (rr : symbol_reference_and_reloc_site ) => (size_of_def rr, (fun (s : nat ) => fun (a : Z ) => fun (e : nat ) => e)) (* FIXME *)))))
+    | "R_X86_64_JUMP_SLOT" =>       (false, (fun (img3 : annotated_memory_image (any_abi_feature )) => (fun (site_addr : nat ) => (fun (rr : symbol_reference_and_reloc_site ) => ( 4 (* CHECK *), (fun (s : nat ) => fun (a : Z ) => fun (e : nat ) => e)) (* FIXME *)))))
+    | "R_X86_64_RELATIVE" =>        (true,  (fun (img3 : annotated_memory_image (any_abi_feature )) => (fun (site_addr : nat ) => (fun (rr : symbol_reference_and_reloc_site ) => ( 8, (fun (s : nat ) => fun (a : Z ) => fun (e : nat ) => e)) (* FIXME *)))))
+    | "R_X86_64_GOTPCREL" =>        (false, (fun (img3 : annotated_memory_image (any_abi_feature )) => (fun (site_addr : nat ) => (fun (rr : symbol_reference_and_reloc_site ) => ( 4, (fun (s : nat ) => fun (a : Z ) => fun (e : nat ) => i2n_signed( 32) ( Coq.ZArith.BinInt.Zminus (Coq.ZArith.BinInt.Zplus(n2i (amd64_got_slot_addr img3 rr)) a) (n2i site_addr)))) )))) 
+    | "R_X86_64_32" =>              (true,  (fun (img3 : annotated_memory_image (any_abi_feature )) => (fun (site_addr : nat ) => (fun (rr : symbol_reference_and_reloc_site ) => ( 4, (fun (s : nat ) => fun (a : Z ) => fun (e : nat ) => i2n ( Coq.ZArith.BinInt.Zplus(n2i s) a)))))))
+    | "R_X86_64_32S" =>             (true,  (fun (img3 : annotated_memory_image (any_abi_feature )) => (fun (site_addr : nat ) => (fun (rr : symbol_reference_and_reloc_site ) => ( 4, (fun (s : nat ) => fun (a : Z ) => fun (e : nat ) => i2n_signed( 32) ( Coq.ZArith.BinInt.Zplus(n2i s) a)))))))
+    | "R_X86_64_16" =>              (true,  (fun (img3 : annotated_memory_image (any_abi_feature )) => (fun (site_addr : nat ) => (fun (rr : symbol_reference_and_reloc_site ) => ( 2, (fun (s : nat ) => fun (a : Z ) => fun (e : nat ) => e)) (* FIXME *)))))
+    | "R_X86_64_PC16" =>            (false, (fun (img3 : annotated_memory_image (any_abi_feature )) => (fun (site_addr : nat ) => (fun (rr : symbol_reference_and_reloc_site ) => ( 2, (fun (s : nat ) => fun (a : Z ) => fun (e : nat ) => e)) (* FIXME *)))))
+    | "R_X86_64_8" =>               (true,  (fun (img3 : annotated_memory_image (any_abi_feature )) => (fun (site_addr : nat ) => (fun (rr : symbol_reference_and_reloc_site ) => ( 1, (fun (s : nat ) => fun (a : Z ) => fun (e : nat ) => e)) (* FIXME *)))))
+    | "R_X86_64_PC8" =>             (false, (fun (img3 : annotated_memory_image (any_abi_feature )) => (fun (site_addr : nat ) => (fun (rr : symbol_reference_and_reloc_site ) => ( 1, (fun (s : nat ) => fun (a : Z ) => fun (e : nat ) => e)) (* FIXME *)))))
+    | "R_X86_64_DTPMOD64" =>        (false, (fun (img3 : annotated_memory_image (any_abi_feature )) => (fun (site_addr : nat ) => (fun (rr : symbol_reference_and_reloc_site ) => ( 8 (* CHECK *), (fun (s : nat ) => fun (a : Z ) => fun (e : nat ) => e)) (* FIXME *)))))
+    | "R_X86_64_DTPOFF64" =>        (false, (fun (img3 : annotated_memory_image (any_abi_feature )) => (fun (site_addr : nat ) => (fun (rr : symbol_reference_and_reloc_site ) => ( 8 (* CHECK *), (fun (s : nat ) => fun (a : Z ) => fun (e : nat ) => e)) (* FIXME *)))))
+    | "R_X86_64_TPOFF64" =>         (false, (fun (img3 : annotated_memory_image (any_abi_feature )) => (fun (site_addr : nat ) => (fun (rr : symbol_reference_and_reloc_site ) => ( 8 (* CHECK *), (fun (s : nat ) => fun (a : Z ) => fun (e : nat ) => e)) (* FIXME *)))))
+    | "R_X86_64_TLSGD" =>           (false, (fun (img3 : annotated_memory_image (any_abi_feature )) => (fun (site_addr : nat ) => (fun (rr : symbol_reference_and_reloc_site ) => ( 8 (* CHECK *), (fun (s : nat ) => fun (a : Z ) => fun (e : nat ) => e)) (* FIXME *)))))
+    | "R_X86_64_TLSLD" =>           (false, (fun (img3 : annotated_memory_image (any_abi_feature )) => (fun (site_addr : nat ) => (fun (rr : symbol_reference_and_reloc_site ) => ( 8 (* CHECK *), (fun (s : nat ) => fun (a : Z ) => fun (e : nat ) => e)) (* FIXME *)))))
+    | "R_X86_64_DTPOFF32" =>        (false, (fun (img3 : annotated_memory_image (any_abi_feature )) => (fun (site_addr : nat ) => (fun (rr : symbol_reference_and_reloc_site ) => ( 4 (* CHECK *), (fun (s : nat ) => fun (a : Z ) => fun (e : nat ) => e)) (* FIXME *)))))
+    | "R_X86_64_GOTTPOFF" =>        (false, (fun (img3 : annotated_memory_image (any_abi_feature )) => (fun (site_addr : nat ) => (fun (rr : symbol_reference_and_reloc_site ) => ( 4, (fun (s : nat ) => fun (a : Z ) => fun (e : nat ) => e)) (* FIXME *)))))
+    | "R_X86_64_TPOFF32" =>         (false, (fun (img3 : annotated_memory_image (any_abi_feature )) => (fun (site_addr : nat ) => (fun (rr : symbol_reference_and_reloc_site ) => ( 4 (* CHECK *), (fun (s : nat ) => fun (a : Z ) => fun (e : nat ) => e)) (* FIXME *)))))
+    | "R_X86_64_PC64" =>            (false, (fun (img3 : annotated_memory_image (any_abi_feature )) => (fun (site_addr : nat ) => (fun (rr : symbol_reference_and_reloc_site ) => ( 8, (fun (s : nat ) => fun (a : Z ) => fun (e : nat ) => e)) (* FIXME *)))))
+    | "R_X86_64_GOTOFF64" =>        (false, (fun (img3 : annotated_memory_image (any_abi_feature )) => (fun (site_addr : nat ) => (fun (rr : symbol_reference_and_reloc_site ) => ( 8, (fun (s : nat ) => fun (a : Z ) => fun (e : nat ) => e)) (* FIXME *)))))
+    | "R_X86_64_GOTPC32" =>         (false, (fun (img3 : annotated_memory_image (any_abi_feature )) => (fun (site_addr : nat ) => (fun (rr : symbol_reference_and_reloc_site ) => ( 4, (fun (s : nat ) => fun (a : Z ) => fun (e : nat ) => e)) (* FIXME *)))))
+    | "R_X86_64_SIZE32" =>          (false, (fun (img3 : annotated_memory_image (any_abi_feature )) => (fun (site_addr : nat ) => (fun (rr : symbol_reference_and_reloc_site ) => ( 4, (fun (s : nat ) => fun (a : Z ) => fun (e : nat ) => e)) (* FIXME *)))))
+    | "R_X86_64_SIZE64" =>          (false, (fun (img3 : annotated_memory_image (any_abi_feature )) => (fun (site_addr : nat ) => (fun (rr : symbol_reference_and_reloc_site ) => ( 8, (fun (s : nat ) => fun (a : Z ) => fun (e : nat ) => e)) (* FIXME *)))))
+    | "R_X86_64_GOTPC32_TLSDESC" => (false, (fun (img3 : annotated_memory_image (any_abi_feature )) => (fun (site_addr : nat ) => (fun (rr : symbol_reference_and_reloc_site ) => ( 4 (* CHECK *), (fun (s : nat ) => fun (a : Z ) => fun (e : nat ) => e)) (* FIXME *)))))
+    | "R_X86_64_TLSDESC_CALL" =>    (false, (fun (img3 : annotated_memory_image (any_abi_feature )) => (fun (site_addr : nat ) => (fun (rr : symbol_reference_and_reloc_site ) => ( 4 (* CHECK *), (fun (s : nat ) => fun (a : Z ) => fun (e : nat ) => e)) (* FIXME *)))))
+    | "R_X86_64_TLSDESC" =>         (false, (fun (img3 : annotated_memory_image (any_abi_feature )) => (fun (site_addr : nat ) => (fun (rr : symbol_reference_and_reloc_site ) => ( 8 (* CHECK *), (fun (s : nat ) => fun (a : Z ) => fun (e : nat ) => e)) (* FIXME *)))))
+    | "R_X86_64_IRELATIVE" =>       (true,  (fun (img3 : annotated_memory_image (any_abi_feature )) => (fun (site_addr : nat ) => (fun (rr : symbol_reference_and_reloc_site ) => ( 8 (* CHECK *), (fun (s : nat ) => fun (a : Z ) => fun (e : nat ) => e)) (* FIXME *)))))
+    | _ => DAEMON
+end.
 (* [?]: removed value specification. *)
 
 Definition sysv_amd64_std_abi   : abi (any_abi_feature ):=  
